update the definition of mod_ty

theories/typing/mod_ty.v
@@ -6,38 +6,66 @@ Set Default Proof Using "Type".
 Section mod_ty.
   Context `{!typeG Σ}.
 
-  Program Definition mod_ty {A B} (f: A → B) `{!Inj (=) (=) f} (ty: type B) : type A := {|
-    ty_size := ty.(ty_size);  ty_lfts := ty.(ty_lfts);  ty_E := ty.(ty_E);
-    ty_own vπd tid vl := ty.(ty_own) (f ∘ vπd.1, vπd.2) tid vl;
-    ty_shr vπd κ tid l := ty.(ty_shr) (f ∘ vπd.1, vπd.2) κ tid l;
-  |}%I.
-  Next Obligation. move=> *. apply ty_size_eq. Qed.
-  Next Obligation. move=> *. by apply ty_own_depth_mono. Qed.
-  Next Obligation. move=> *. by apply ty_shr_depth_mono. Qed.
-  Next Obligation. move=> *. apply ty_shr_lft_mono. Qed.
-  Next Obligation.  move=> *. by apply ty_share. Qed.
-  Next Obligation.
-    move=> */=. iIntros "#LFT In Own Tok".
-    iMod (ty_own_proph with "LFT In Own Tok") as "Upd"; [done|].
-    iApply (step_fupdN_wand with "Upd"). iModIntro. iMod 1 as (ξs q ?) "[PTok Close]".
-    iModIntro. iExists ξs, q. iSplit; [iPureIntro; by apply (proph_dep_destr _)|iFrame].
-  Qed.
-  Next Obligation.
-    move=> */=. iIntros "#LFT In In' Shr Tok".
-    iMod (ty_shr_proph with "LFT In In' Shr Tok") as "Upd"; [done|]. iIntros "!>!>".
-    iApply (step_fupdN_wand with "Upd"). iMod 1 as (ξs q ?) "[PTok Close]".
-    iModIntro. iExists ξs, q. iSplit; [iPureIntro; by apply (proph_dep_destr _)|iFrame].
+  Local Lemma mod_ty_mt {A B} (f: A → B) ty vπ' d tid l q :
+    (l ↦∗{q}: λ vl, ∃vπ, ⌜vπ' = f ∘ vπ⌝ ∗ ty.(ty_own) (vπ,d) tid vl)%I ⊣⊢
+    ∃vπ, ⌜vπ' = f ∘ vπ⌝ ∗ l ↦∗{q}: ty.(ty_own) (vπ,d) tid.
+  Proof. iSplit.
+    - iDestruct 1 as (vl) "[Mt Own]". iDestruct "Own" as (vπ->) "Own".
+      iExists vπ. iSplit; [done|]. iExists vl. iFrame.
+    - iDestruct 1 as (vπ->vl) "[Mt Own]". iExists vl. iFrame "Mt". iExists vπ.
+      by iSplit; [done|].
   Qed.
 
-  Global Instance mod_ty_type_nonexpansive `{Inj A B (=) (=) f} :
-    TypeNonExpansive (mod_ty f).
-  Proof. split; [|done|by move=> */=|by move=> */=].
+  Program Definition mod_ty {A B} (f: A → B) (ty: type A) : type B := {|
+    ty_size := ty.(ty_size);  ty_lfts := ty.(ty_lfts);  ty_E := ty.(ty_E);
+    ty_own vπd tid vl := ∃vπ, ⌜vπd.1 = f ∘ vπ⌝ ∗ ty.(ty_own) (vπ,vπd.2) tid vl;
+    ty_shr vπd κ tid l := ∃vπ, ⌜vπd.1 = f ∘ vπ⌝ ∗ ty.(ty_shr) (vπ,vπd.2) κ tid l;
+  |}%I.
+  Next Obligation. move=> *. iDestruct 1 as (??) "?". by iApply ty_size_eq. Qed.
+  Next Obligation.
+    move=> */=. iDestruct 1 as (vπ->) "?". iExists vπ. iSplit; [done|].
+    by iApply ty_own_depth_mono.
+  Qed.
+  Next Obligation.
+    move=> */=. iDestruct 1 as (vπ->) "?". iExists vπ. iSplit; [done|].
+    by iApply ty_shr_depth_mono.
+  Qed.
+  Next Obligation.
+    move=> */=. iIntros "#?". iDestruct 1 as (vπ->) "?". iExists vπ. iSplit; [done|].
+    by iApply ty_shr_lft_mono.
+  Qed.
+  Next Obligation.
+    move=> */=. iIntros "#LFT In Bor Tok". rewrite mod_ty_mt.
+    iMod (bor_exists_tok with "LFT Bor Tok") as (vπ) "[Bor Tok]"; [done|].
+    iMod (bor_sep_persistent with "LFT Bor Tok") as "[>->[Bor Tok]]"; [done|].
+    iMod (ty_share with "LFT In Bor Tok") as "Upd"; [done|].
+    iApply (step_fupdN_wand with "Upd"). iIntros "!> >[Shr $] !>". iExists vπ. by iSplit.
+  Qed.
+  Next Obligation.
+    move=> */=. iIntros "#LFT In". iDestruct 1 as (vπ->) "Own". iIntros "Tok".
+    iMod (ty_own_proph with "LFT In Own Tok") as "Upd"; [done|]. iModIntro.
+    iApply (step_fupdN_wand with "Upd"). iMod 1 as (ξs q ?) "[PTok Close]".
+    iModIntro. iExists ξs, q. iSplit; [iPureIntro; by apply (proph_dep_constr _)|].
+    iFrame "PTok". iIntros "PTok". iMod ("Close" with "PTok") as "[Own $]".
+    iModIntro. iExists vπ. by iSplit.
+  Qed.
+  Next Obligation.
+    move=> */=. iIntros "#LFT In In'". iDestruct 1 as (vπ->) "Shr". iIntros "Tok".
+    iMod (ty_shr_proph with "LFT In In' Shr Tok") as "Upd"; [done|]. iIntros "!>!>".
+    iApply (step_fupdN_wand with "Upd"). iMod 1 as (ξs q ?) "[PTok Close]".
+    iModIntro. iExists ξs, q. iSplit; [iPureIntro; by apply (proph_dep_constr _)|].
+    iFrame "PTok". iIntros "PTok". iMod ("Close" with "PTok") as "[Own $]".
+    iModIntro. iExists vπ. by iSplit.
+  Qed.
+
+  Global Instance mod_ty_type_nonexpansive {A B} (f: A → B) : TypeNonExpansive (mod_ty f).
+  Proof. split; [|done|move=> */=; by do 3 f_equiv|move=> */=; by do 3 f_equiv].
     apply (type_lft_morphism_add _ static [] [])=> ?.
     - rewrite left_id. apply lft_equiv_refl.
     - by rewrite /elctx_interp /= left_id right_id.
   Qed.
 
-  Global Instance mod_ty_ne `{Inj A B (=) (=) f} : NonExpansive (mod_ty f).
+  Global Instance mod_ty_ne {A B} (f: A → B) : NonExpansive (mod_ty f).
   Proof. solve_ne_type. Qed.
 
 End mod_ty.
@@ -45,47 +73,48 @@ End mod_ty.
 Section typing.
   Context `{!typeG Σ}.
 
-  Global Instance mod_ty_copy `{Inj A B (=) (=) f} ty : Copy ty → Copy (mod_ty f ty).
+  Global Instance mod_ty_copy {A B} (f: A → B) ty : Copy ty → Copy (mod_ty f ty).
   Proof.
-    move=> [? ShrAcc]. split; [by apply _|]. move=> */=. iIntros "LFT Shr Na Tok".
-    iMod (ShrAcc with "LFT Shr Na Tok") as (q vl) "[$[Mt[Own Close]]]"; [done|done|].
-    iModIntro. iExists q, vl. iFrame.
+    move=> [? ShrAcc]. split; [by apply _|]. move=> */=. iIntros "LFT".
+    iDestruct 1 as (vπ ->) "Shr". iIntros "Na Tok".
+    iMod (ShrAcc with "LFT Shr Na Tok") as (q vl) "[$[Mt[? Close]]]"; [done|done|].
+    iModIntro. iExists q, vl. iFrame "Mt Close". iNext. iExists vπ. by iSplit.
   Qed.
 
-  Global Instance mod_ty_send `{Inj A B (=) (=) f} ty : Send ty → Send (mod_ty f ty).
-  Proof. by move=> ??*/=. Qed.
+  Global Instance mod_ty_send {A B} (f: A → B) ty : Send ty → Send (mod_ty f ty).
+  Proof. move=> ??*/=. by do 3 f_equiv. Qed.
 
-  Global Instance mod_ty_sync `{Inj A B (=) (=) f} ty : Sync ty → Sync (mod_ty f ty).
-  Proof. by move=> ??*/=. Qed.
+  Global Instance mod_ty_sync {A B} (f: A → B) ty : Sync ty → Sync (mod_ty f ty).
+  Proof. move=> ??*/=. by do 3 f_equiv. Qed.
 
-  Lemma mod_ty_subtype_out `{Inj A B (=) (=) f} E L ty : subtype E L f (mod_ty f ty) ty.
+  Lemma mod_ty_subtype_in {A B} E L (f: A → B) ty : subtype E L f ty (mod_ty f ty).
   Proof.
     iIntros "*_!>_". iSplit; [done|]. iSplit; [by iApply lft_incl_refl|].
-    iSplit; by iIntros "!>*?".
+    iSplit; iIntros "!>" (vπ) "*?"; iExists vπ; by iSplit.
   Qed.
 
-  Lemma mod_ty_subtype_in `{Inj A B (=) (=) f} E L g ty :
-    f ∘ g = id → subtype E L g ty (mod_ty f ty).
+  Lemma mod_ty_subtype_out {A B} E L (f: A → B) g ty :
+    g ∘ f = id → subtype E L g (mod_ty f ty) ty.
   Proof.
     move=> Eq. iIntros "*_!>_". iSplit; [done|]. iSplit; [by iApply lft_incl_refl|].
-    iSplit; iIntros "!>*?/="; by rewrite compose_assoc Eq.
+    iSplit; iIntros "!>*/="; iDestruct 1 as (vπ'->) "?"; by rewrite compose_assoc Eq.
   Qed.
 
-  Lemma mod_ty_eqtype_inout `{Inj A B (=) (=) f} E L g ty :
-    f ∘ g = id → eqtype E L g f ty (mod_ty f ty).
+  Lemma mod_ty_eqtype_inout {A B} E L (f: A → B) g ty :
+    g ∘ f = id → eqtype E L f g ty (mod_ty f ty).
   Proof. move=> ?. by split; [apply mod_ty_subtype_in|apply mod_ty_subtype_out]. Qed.
 
-  Lemma mod_ty_subtype `{Inj A B (=) (=) f, Inj A' B' (=) (=) f'} E L h g' ty ty' :
-    f' ∘ g' = id → subtype E L h ty ty' →
-    subtype E L (g' ∘ h ∘ f) (mod_ty f ty) (mod_ty f' ty').
+  Lemma mod_ty_subtype {A B A' B'} E L h (f: A → B) (f': A' → B') g ty ty' :
+    g ∘ f = id → subtype E L h ty ty' →
+    subtype E L (f' ∘ h ∘ g) (mod_ty f ty) (mod_ty f' ty').
   Proof.
     move=> ??. eapply subtype_trans; [by apply mod_ty_subtype_out|].
     eapply subtype_trans; by [|apply mod_ty_subtype_in].
   Qed.
 
-  Lemma mod_ty_eqtype `{Inj A B (=) (=) f, Inj A' B' (=) (=) f'} E L h h' g g' ty ty' :
-    f ∘ g = id → f' ∘ g' = id → eqtype E L h h' ty ty' →
-    eqtype E L (g' ∘ h ∘ f) (g ∘ h' ∘ f') (mod_ty f ty) (mod_ty f' ty').
+  Lemma mod_ty_eqtype {A B A' B'} E L h h' (f: A → B) (f': A' → B') g g' ty ty' :
+    g ∘ f = id → g' ∘ f' = id → eqtype E L h h' ty ty' →
+    eqtype E L (f' ∘ h ∘ g) (f ∘ h' ∘ g') (mod_ty f ty) (mod_ty f' ty').
   Proof. move=> ??[??]. split; by apply mod_ty_subtype. Qed.
 
 End typing.
